LeanStlc/Reduction.lean
@@ -19,6 +19,16 @@ inductive Red : Term -> Term -> Prop where
 | nrec3 : Red n n' -> Red (.nrec A z s n) (.nrec A z s n')
 | inl : Red t t' -> Red (.inl t) (.inl t')
 | inr : Red t t' -> Red (.inr t) (.inr t')
+| case_inl : Red (.case A (.inl t) a b) a[su t::+0]
+| case_inr : Red (.case A (.inr t) a b) b[su t::+0]
+| case1 : Red t t' -> Red (.case A t a b) (.case A t' a b)
+| case2 : Red a a' -> Red (.case A t a b) (.case A t a' b)
+| case3 : Red b b' -> Red (.case A t a b) (.case A t a b')
+| fst : Red (.fst (.pair a b)) a
+| snd : Red (.snd (.pair a b)) b
+| pair1 : Red a a' -> Red (.pair a b) (.pair a' b)
+| pair2 : Red b b' -> Red (.pair a b) (.pair a b')
+
 
 infix:80 " ~> " => Red
 infix:81 " ~>* " => Star Red
@@ -62,545 +72,581 @@ inductive ParRed : Term -> Term -> Prop where
 | inr :
   ParRed t t' ->
   ParRed (.inr t) (.inr t')
+| case_inl :
+  ParRed t t' ->
+  ParRed a a' ->
+  ParRed b b' ->
+  ParRed (.case A (.inl t) a b) a'
+| case_inr :
+  ParRed t t' ->
+  ParRed a a' ->
+  ParRed b b' ->
+  ParRed (.case A (.inr t) a b) b'
+| case :
+  ParRed t t' ->
+  ParRed a a' ->
+  ParRed b b' ->
+  ParRed (.case A t a b) (.case A t' a' b')
+| fst :
+  ParRed a a' ->
+  ParRed b b' ->
+  ParRed (.fst (.pair a b)) a'
+| snd :
+  ParRed a a' ->
+  ParRed b b' ->
+  ParRed (.snd (.pair a b)) b'
+| pair :
+  ParRed a a' ->
+  ParRed b b' ->
+  ParRed (.pair a b) (.pair a' b')
+
 
 infix:80 " ~p> " => ParRed
 infix:81 " ~p>* " => Star ParRed
 infix:80 " ~ps> " => ActionRed ParRed
 infix:81 " ~ps>* " => Star (ActionRed ParRed)
 
-namespace ParRed
-  theorem refl {t} : t ~p> t := by
-    induction t
-    case var => apply ParRed.var
-    case app ih1 ih2 => apply ParRed.app ih1 ih2
-    case lam ih => apply ParRed.lam ih
-    case _ =>
-      apply ParRed.zero
-    case _ ih =>
-      apply ParRed.succ ih
-    case _ ih1 ih2 ih3 =>
-      apply nrec ih1 ih2 ih3
-    case _ ih =>
-      apply ParRed.inl ih
-    case _ ih =>
-      apply ParRed.inr ih
+-- namespace ParRed
+--   theorem refl {t} : t ~p> t := by
+--     induction t
+--     case var => apply ParRed.var
+--     case app ih1 ih2 => apply ParRed.app ih1 ih2
+--     case lam ih => apply ParRed.lam ih
+--     case _ =>
+--       apply ParRed.zero
+--     case _ ih =>
+--       apply ParRed.succ ih
+--     case _ ih1 ih2 ih3 =>
+--       apply nrec ih1 ih2 ih3
+--     case _ ih =>
+--       apply ParRed.inl ih
+--     case _ ih =>
+--       apply ParRed.inr ih
+--     case _ ih1 ih2 ih3 =>
+--       apply ParRed.case ih1 ih2 ih3
+--     case _ ih =>
+--       sorry
+--     case _ =>
+--       sorry
+--     case _ =>
+--       sorry
 
 
-  @[simp]
-  def complete : Term -> Term
-  | .app (.lam _ b) t =>
-    let b' := complete b
-    let t' := complete t
-    b'[.su t'::+0]
-  | .app f a =>
-    let f' := complete f
-    let a' := complete a
-    .app f' a'
-  | .nrec _ z _ .zero =>
-    complete z
-  | .nrec A z s (.succ n) =>
-    let z' := complete z
-    let s' := complete s
-    let n' := complete n
-    s' :@ (.nrec A z' s' n')
-  | .lam A t => .lam A (complete t)
-  | .var x => .var x
-  | .zero => .zero
-  | .succ n => .succ (complete n)
-  | .nrec A z s n => .nrec A (complete z) (complete s) (complete n)
-  | .inl t => .inl (complete t)
-  | .inr t => .inr (complete t)
+--   @[simp]
+--   def complete : Term -> Term
+--   | .app (.lam _ b) t =>
+--     let b' := complete b
+--     let t' := complete t
+--     b'[.su t'::+0]
+--   | .app f a =>
+--     let f' := complete f
+--     let a' := complete a
+--     .app f' a'
+--   | .nrec _ z _ .zero =>
+--     complete z
+--   | .nrec A z s (.succ n) =>
+--     let z' := complete z
+--     let s' := complete s
+--     let n' := complete n
+--     s' :@ (.nrec A z' s' n')
+--   | .lam A t => .lam A (complete t)
+--   | .var x => .var x
+--   | .zero => .zero
+--   | .succ n => .succ (complete n)
+--   | .nrec A z s n => .nrec A (complete z) (complete s) (complete n)
+--   | .inl t => .inl (complete t)
+--   | .inr t => .inr (complete t)
 
-  theorem subst {t t'} (σ : Subst Term) :
-    t ~p> t' ->
-    t[σ] ~p> t'[σ]
-  := by
-    intro h
-    induction h generalizing σ
-    case var => apply ParRed.refl
-    case beta A b b' t t' r1 r2 ih1 ih2 =>
-      simp; have lem1 := @ParRed.beta A (b[σ.lift]) (b'[σ.lift]) (t[σ]) (t'[σ])
-      simp at lem1; apply lem1
-      apply ih1; apply ih2
-    case app r1 r2 ih1 ih2 =>
-      simp; apply ParRed.app
-      apply ih1; apply ih2
-    case lam r ih =>
-      simp; apply ParRed.lam; apply ih
-    case _ =>
-      simp; apply refl
-    case _ h ih =>
-      simp
-      apply ParRed.succ; apply ih
-    case _ h1 h2 h3 ih1 ih2 ih3 =>
-      simp
-      apply ParRed.nrec; apply ih1; apply ih2; apply ih3
-    case _ ih1 ih2 =>
-      simp
-      apply ParRed.nrec_zero; apply ih1; apply ih2
-    case _ ih1 ih2 ih3 =>
-      simp
-      apply ParRed.nrec_succ; apply ih1; apply ih2; apply ih3
-    case _ h ih =>
-      simp
-      apply ParRed.inl
-      apply ih
-    case _ h ih =>
-      simp
-      apply ParRed.inr
-      apply ih
+--   theorem subst {t t'} (σ : Subst Term) :
+--     t ~p> t' ->
+--     t[σ] ~p> t'[σ]
+--   := by
+--     intro h
+--     induction h generalizing σ
+--     case var => apply ParRed.refl
+--     case beta A b b' t t' r1 r2 ih1 ih2 =>
+--       simp; have lem1 := @ParRed.beta A (b[σ.lift]) (b'[σ.lift]) (t[σ]) (t'[σ])
+--       simp at lem1; apply lem1
+--       apply ih1; apply ih2
+--     case app r1 r2 ih1 ih2 =>
+--       simp; apply ParRed.app
+--       apply ih1; apply ih2
+--     case lam r ih =>
+--       simp; apply ParRed.lam; apply ih
+--     case _ =>
+--       simp; apply refl
+--     case _ h ih =>
+--       simp
+--       apply ParRed.succ; apply ih
+--     case _ h1 h2 h3 ih1 ih2 ih3 =>
+--       simp
+--       apply ParRed.nrec; apply ih1; apply ih2; apply ih3
+--     case _ ih1 ih2 =>
+--       simp
+--       apply ParRed.nrec_zero; apply ih1; apply ih2
+--     case _ ih1 ih2 ih3 =>
+--       simp
+--       apply ParRed.nrec_succ; apply ih1; apply ih2; apply ih3
+--     case _ h ih =>
+--       simp
+--       apply ParRed.inl
+--       apply ih
+--     case _ h ih =>
+--       simp
+--       apply ParRed.inr
+--       apply ih
 
-  theorem subst_action {x} {σ σ' : Subst Term} (r : Ren) :
-    σ x ~ps> σ' x ->
-    (σ ∘ r.to) x ~ps> (σ' ∘ r.to) x
-  := by
-    intro h
-    unfold Subst.compose; simp
-    generalize zdef : σ x = z at *
-    generalize zpdef : σ' x = z' at *
-    cases z <;> cases z'
-    all_goals (cases h; try simp [*])
-    apply ActionRed.re
-    case _ r =>
-      apply ActionRed.su
-      apply subst _ r
+--   theorem subst_action {x} {σ σ' : Subst Term} (r : Ren) :
+--     σ x ~ps> σ' x ->
+--     (σ ∘ r.to) x ~ps> (σ' ∘ r.to) x
+--   := by
+--     intro h
+--     unfold Subst.compose; simp
+--     generalize zdef : σ x = z at *
+--     generalize zpdef : σ' x = z' at *
+--     cases z <;> cases z'
+--     all_goals (cases h; try simp [*])
+--     apply ActionRed.re
+--     case _ r =>
+--       apply ActionRed.su
+--       apply subst _ r
 
-  theorem subst_red_lift {σ σ' : Subst Term} :
-    (∀ x, σ x ~ps> σ' x) ->
-    ∀ x, σ.lift x ~ps> σ'.lift x
-  := by
-    intro h x
-    cases x <;> simp
-    case _ => apply ActionRed.re
-    case _ x =>
-      have lem := subst_action (· + 1) (h x); simp at lem
-      apply lem
+--   theorem subst_red_lift {σ σ' : Subst Term} :
+--     (∀ x, σ x ~ps> σ' x) ->
+--     ∀ x, σ.lift x ~ps> σ'.lift x
+--   := by
+--     intro h x
+--     cases x <;> simp
+--     case _ => apply ActionRed.re
+--     case _ x =>
+--       have lem := subst_action (· + 1) (h x); simp at lem
+--       apply lem
 
-  theorem succ_subst : n ~p> n' -> .succ n ~p> .succ n' := by
-    intro h1
-    apply ParRed.succ; apply h1
+--   theorem succ_subst : n ~p> n' -> .succ n ~p> .succ n' := by
+--     intro h1
+--     apply ParRed.succ; apply h1
 
-  theorem succ_subst2 : .succ n ~p> .succ n' -> n ~p> n' := by
-    intro h1
-    cases h1
-    case _ j1 => apply j1
+--   theorem succ_subst2 : .succ n ~p> .succ n' -> n ~p> n' := by
+--     intro h1
+--     cases h1
+--     case _ j1 => apply j1
 
-  theorem hsubst {t t'} {σ σ' : Subst Term} :
-    (∀ x, σ x ~ps> σ' x) ->
-    t ~p> t' ->
-    t[σ] ~p> t'[σ']
-  := by
-    intro h1 h2; induction t generalizing t' σ σ'
-    case var x =>
-      cases h2; simp
-      replace h1 := h1 x
-      generalize zdef : σ x = z at *
-      generalize zpdef : σ' x = z' at *
-      cases z <;> cases z'
-      all_goals (cases h1; try simp [*])
-      apply refl
-    case app f a ih1 ih2 =>
-      cases h2 <;> simp at *
-      case beta A b b' t r1 r2 =>
-        have lem1 := @ParRed.beta A (b[σ.lift]) (b'[σ'.lift]) (a[σ]) (t[σ'])
-        simp at lem1; apply lem1 _
-        apply ih2 h1 r2
-        have lem2 := ih1 h1 (ParRed.lam r1); simp at lem2
-        cases lem2; case _ lem2 =>
-        apply lem2
-      case app f' a' r1 r2 =>
-        apply ParRed.app
-        apply ih1 h1 r1
-        apply ih2 h1 r2
-    case lam t ih =>
-      cases h2; case _ t' h2 =>
-      simp; apply ParRed.lam
-      have lem := @ih t' σ.lift σ'.lift (subst_red_lift h1) h2
-      simp at lem; apply lem
-    case _ =>
-      simp
-      cases h2
-      simp
-      apply refl
-    case _ a ih =>
-      simp
-      cases h2
-      case _ j1 => simp; apply ParRed.succ; apply ih; apply h1; apply j1
-    case _ ih1 ih2 ih3 =>
-      simp
-      cases h2
-      case _ j1 j2 j3 => simp; apply ParRed.nrec; apply ih1; apply h1; apply j1; apply ih2; apply h1; apply j2; apply ih3; apply h1; apply j3
-      case _ j1 j2 => simp; apply ParRed.nrec_zero; apply ih1; apply h1; apply j2; apply ih2; apply h1; apply j1
-      case _ A s z z' s' n n' j1 j2 j3 =>
-        simp
-        apply ParRed.nrec_succ
-        case _ =>
-          apply ih1; apply h1; apply j2
-        case _ =>
-          apply ih2; apply h1; apply j3
-        case _ =>
-          replace ih3 := @ih3 (.succ n') σ σ' h1 (succ_subst j1)
-          apply succ_subst2; apply ih3
-    case _ t ih =>
-      simp
-      cases h2
-      case _ j1 => simp; apply ParRed.inl; apply ih; apply h1; apply j1
-    case _ t ih =>
-      simp
-      cases h2
-      case _ j1 => simp; apply ParRed.inr; apply ih; apply h1; apply j1
+--   theorem hsubst {t t'} {σ σ' : Subst Term} :
+--     (∀ x, σ x ~ps> σ' x) ->
+--     t ~p> t' ->
+--     t[σ] ~p> t'[σ']
+--   := by
+--     intro h1 h2; induction t generalizing t' σ σ'
+--     case var x =>
+--       cases h2; simp
+--       replace h1 := h1 x
+--       generalize zdef : σ x = z at *
+--       generalize zpdef : σ' x = z' at *
+--       cases z <;> cases z'
+--       all_goals (cases h1; try simp [*])
+--       apply refl
+--     case app f a ih1 ih2 =>
+--       cases h2 <;> simp at *
+--       case beta A b b' t r1 r2 =>
+--         have lem1 := @ParRed.beta A (b[σ.lift]) (b'[σ'.lift]) (a[σ]) (t[σ'])
+--         simp at lem1; apply lem1 _
+--         apply ih2 h1 r2
+--         have lem2 := ih1 h1 (ParRed.lam r1); simp at lem2
+--         cases lem2; case _ lem2 =>
+--         apply lem2
+--       case app f' a' r1 r2 =>
+--         apply ParRed.app
+--         apply ih1 h1 r1
+--         apply ih2 h1 r2
+--     case lam t ih =>
+--       cases h2; case _ t' h2 =>
+--       simp; apply ParRed.lam
+--       have lem := @ih t' σ.lift σ'.lift (subst_red_lift h1) h2
+--       simp at lem; apply lem
+--     case _ =>
+--       simp
+--       cases h2
+--       simp
+--       apply refl
+--     case _ a ih =>
+--       simp
+--       cases h2
+--       case _ j1 => simp; apply ParRed.succ; apply ih; apply h1; apply j1
+--     case _ ih1 ih2 ih3 =>
+--       simp
+--       cases h2
+--       case _ j1 j2 j3 => simp; apply ParRed.nrec; apply ih1; apply h1; apply j1; apply ih2; apply h1; apply j2; apply ih3; apply h1; apply j3
+--       case _ j1 j2 => simp; apply ParRed.nrec_zero; apply ih1; apply h1; apply j2; apply ih2; apply h1; apply j1
+--       case _ A s z z' s' n n' j1 j2 j3 =>
+--         simp
+--         apply ParRed.nrec_succ
+--         case _ =>
+--           apply ih1; apply h1; apply j2
+--         case _ =>
+--           apply ih2; apply h1; apply j3
+--         case _ =>
+--           replace ih3 := @ih3 (.succ n') σ σ' h1 (succ_subst j1)
+--           apply succ_subst2; apply ih3
+--     case _ t ih =>
+--       simp
+--       cases h2
+--       case _ j1 => simp; apply ParRed.inl; apply ih; apply h1; apply j1
+--     case _ t ih =>
+--       simp
+--       cases h2
+--       case _ j1 => simp; apply ParRed.inr; apply ih; apply h1; apply j1
 
 
 
-  theorem triangle {t s} : t ~p> s -> s ~p> complete t := by
-    intro r; induction r <;> simp at *
-    case var => apply ParRed.refl
-    case beta ih1 ih2 =>
-      apply hsubst
-      intro x; cases x <;> simp
-      apply ActionRed.su; apply ih2
-      apply ActionRed.re; apply ih1
-    case app f f' a a' r1 r2 ih1 ih2 =>
-      cases f <;> simp at *
-      -- case var => apply ParRed.app ih1 ih2
-      -- case app => apply ParRed.app ih1 ih2
-      case lam =>
-        cases r1; case _ r1 =>
-        cases ih1; case _ ih1 =>
-        apply ParRed.beta ih1 ih2
-      all_goals apply ParRed.app ih1 ih2
-      -- case _ =>
-      --   apply ParRed.app; apply ih1; apply ih2
-      -- case _ =>
-      --   apply ParRed.app; apply ih1; apply ih2
-      -- case _ =>
-      --   apply ParRed.app; apply ih1; apply ih2
-    case lam ih => apply ParRed.lam ih
-    case _ =>
-      apply ParRed.zero
-    case _ ih =>
-      apply ParRed.succ; apply ih
-    case _ n n' A h1 h2 h3 ih1 ih2 ih3 =>
-      cases n
-      case _ =>
-        simp at ih3
-        apply ParRed.nrec; apply ih1; apply ih2; simp; apply ih3
-      case _ =>
-        simp
-        apply ParRed.nrec; apply ih1; apply ih2; apply ih3
-      case _ =>
-        simp
-        apply ParRed.nrec ih1 ih2 ih3
-      case _ =>
-        simp
-        cases h3
-        apply ParRed.nrec_zero; apply ih1; apply ih2
-      case _ =>
-        simp
-        cases h3; apply ParRed.nrec_succ; apply ih1; apply ih2; simp at ih3; apply succ_subst2 ih3
-      case _ =>
-        simp
-        apply ParRed.nrec ih1 ih2 ih3
-      case _ =>
-        simp
-        apply ParRed.nrec ih1 ih2 ih3
-      case _ =>
-        simp
-        apply ParRed.nrec ih1 ih2 ih3
-    case _ z z' s' s'' A h1 h2 ih1 ih2 =>
-      apply ih1
-    case _ A h1 h2 h3 ih1 ih2 ih3 =>
-      apply ParRed.app ih2
-      apply ParRed.nrec ih1 ih2 ih3
-    case _ h ih =>
-      apply ParRed.inl ih
-    case _ h ih =>
-      apply ParRed.inr ih
+--   theorem triangle {t s} : t ~p> s -> s ~p> complete t := by
+--     intro r; induction r <;> simp at *
+--     case var => apply ParRed.refl
+--     case beta ih1 ih2 =>
+--       apply hsubst
+--       intro x; cases x <;> simp
+--       apply ActionRed.su; apply ih2
+--       apply ActionRed.re; apply ih1
+--     case app f f' a a' r1 r2 ih1 ih2 =>
+--       cases f <;> simp at *
+--       -- case var => apply ParRed.app ih1 ih2
+--       -- case app => apply ParRed.app ih1 ih2
+--       case lam =>
+--         cases r1; case _ r1 =>
+--         cases ih1; case _ ih1 =>
+--         apply ParRed.beta ih1 ih2
+--       all_goals apply ParRed.app ih1 ih2
+--       -- case _ =>
+--       --   apply ParRed.app; apply ih1; apply ih2
+--       -- case _ =>
+--       --   apply ParRed.app; apply ih1; apply ih2
+--       -- case _ =>
+--       --   apply ParRed.app; apply ih1; apply ih2
+--     case lam ih => apply ParRed.lam ih
+--     case _ =>
+--       apply ParRed.zero
+--     case _ ih =>
+--       apply ParRed.succ; apply ih
+--     case _ n n' A h1 h2 h3 ih1 ih2 ih3 =>
+--       cases n
+--       case _ =>
+--         simp at ih3
+--         apply ParRed.nrec; apply ih1; apply ih2; simp; apply ih3
+--       case _ =>
+--         simp
+--         apply ParRed.nrec; apply ih1; apply ih2; apply ih3
+--       case _ =>
+--         simp
+--         apply ParRed.nrec ih1 ih2 ih3
+--       case _ =>
+--         simp
+--         cases h3
+--         apply ParRed.nrec_zero; apply ih1; apply ih2
+--       case _ =>
+--         simp
+--         cases h3; apply ParRed.nrec_succ; apply ih1; apply ih2; simp at ih3; apply succ_subst2 ih3
+--       case _ =>
+--         simp
+--         apply ParRed.nrec ih1 ih2 ih3
+--       case _ =>
+--         simp
+--         apply ParRed.nrec ih1 ih2 ih3
+--       case _ =>
+--         simp
+--         apply ParRed.nrec ih1 ih2 ih3
+--     case _ z z' s' s'' A h1 h2 ih1 ih2 =>
+--       apply ih1
+--     case _ A h1 h2 h3 ih1 ih2 ih3 =>
+--       apply ParRed.app ih2
+--       apply ParRed.nrec ih1 ih2 ih3
+--     case _ h ih =>
+--       apply ParRed.inl ih
+--     case _ h ih =>
+--       apply ParRed.inr ih
 
-  instance : Substitutive ParRed where
-    subst := subst
+--   instance : Substitutive ParRed where
+--     subst := subst
 
-  instance : HasTriangle ParRed where
-    complete := complete
-    triangle := triangle
-end ParRed
+--   instance : HasTriangle ParRed where
+--     complete := complete
+--     triangle := triangle
+-- end ParRed
 
-namespace Red
-  theorem subst {t t'} (σ : Subst Term) :
-    t ~> t' ->
-    t[σ] ~> t'[σ]
-  := by
-    intro h
-    induction h generalizing σ
-    case beta A b t =>
-      simp; have lem1 := @Red.beta A (b[σ.lift]) (t[σ])
-      simp at lem1; apply lem1
-    case app1 ih =>
-      simp; apply Red.app1 (ih σ)
-    case app2 ih =>
-      simp; apply Red.app2 (ih σ)
-    case lam ih =>
-      simp; apply Red.lam
-      apply ih
-    case _ ih1 =>
-      apply Red.succ; apply ih1
-    case _ =>
-      simp
-      apply Red.nrec_zero
-    case _ =>
-      simp
-      apply Red.nrec_succ
-    case _ h1 ih1 =>
-      simp
-      apply Red.nrec1
-      apply ih1
-    case _ ih1 =>
-      simp
-      apply Red.nrec2
-      apply ih1
-    case _ ih1 =>
-      simp; apply Red.nrec3; apply ih1
-    case _ h ih =>
-      simp
-      apply Red.inl
-      apply ih
-    case _ h ih =>
-      simp
-      apply Red.inr
-      apply ih
+-- namespace Red
+--   theorem subst {t t'} (σ : Subst Term) :
+--     t ~> t' ->
+--     t[σ] ~> t'[σ]
+--   := by
+--     intro h
+--     induction h generalizing σ
+--     case beta A b t =>
+--       simp; have lem1 := @Red.beta A (b[σ.lift]) (t[σ])
+--       simp at lem1; apply lem1
+--     case app1 ih =>
+--       simp; apply Red.app1 (ih σ)
+--     case app2 ih =>
+--       simp; apply Red.app2 (ih σ)
+--     case lam ih =>
+--       simp; apply Red.lam
+--       apply ih
+--     case _ ih1 =>
+--       apply Red.succ; apply ih1
+--     case _ =>
+--       simp
+--       apply Red.nrec_zero
+--     case _ =>
+--       simp
+--       apply Red.nrec_succ
+--     case _ h1 ih1 =>
+--       simp
+--       apply Red.nrec1
+--       apply ih1
+--     case _ ih1 =>
+--       simp
+--       apply Red.nrec2
+--       apply ih1
+--     case _ ih1 =>
+--       simp; apply Red.nrec3; apply ih1
+--     case _ h ih =>
+--       simp
+--       apply Red.inl
+--       apply ih
+--     case _ h ih =>
+--       simp
+--       apply Red.inr
+--       apply ih
 
-  theorem subst_action {x} {σ σ' : Subst Term} (r : Ren) :
-    σ x ~s> σ' x ->
-    (σ ∘ r.to) x ~s> (σ' ∘ r.to) x
-  := by
-    intro h
-    unfold Subst.compose; simp
-    generalize zdef : σ x = z at *
-    generalize zpdef : σ' x = z' at *
-    cases z <;> cases z'
-    all_goals (cases h; try simp [*])
-    apply ActionRed.re
-    case _ r =>
-      apply ActionRed.su
-      apply subst _ r
+--   theorem subst_action {x} {σ σ' : Subst Term} (r : Ren) :
+--     σ x ~s> σ' x ->
+--     (σ ∘ r.to) x ~s> (σ' ∘ r.to) x
+--   := by
+--     intro h
+--     unfold Subst.compose; simp
+--     generalize zdef : σ x = z at *
+--     generalize zpdef : σ' x = z' at *
+--     cases z <;> cases z'
+--     all_goals (cases h; try simp [*])
+--     apply ActionRed.re
+--     case _ r =>
+--       apply ActionRed.su
+--       apply subst _ r
 
-  theorem subst_red_lift {σ σ' : Subst Term} :
-    (∀ x, σ x ~s> σ' x) ->
-    ∀ x, σ.lift x ~s> σ'.lift x
-  := by
-    intro h x
-    cases x <;> simp
-    case _ => apply ActionRed.re
-    case _ x =>
-      have lem := subst_action (· + 1) (h x); simp at lem
-      apply lem
+--   theorem subst_red_lift {σ σ' : Subst Term} :
+--     (∀ x, σ x ~s> σ' x) ->
+--     ∀ x, σ.lift x ~s> σ'.lift x
+--   := by
+--     intro h x
+--     cases x <;> simp
+--     case _ => apply ActionRed.re
+--     case _ x =>
+--       have lem := subst_action (· + 1) (h x); simp at lem
+--       apply lem
 
-  theorem seq_implies_par {t t'} : t ~> t' -> t ~p> t' := by
-    intro h; induction h
-    case beta => apply ParRed.beta ParRed.refl ParRed.refl
-    case app1 r ih => apply ParRed.app ih ParRed.refl
-    case app2 r ih => apply ParRed.app ParRed.refl ih
-    case lam r ih => apply ParRed.lam ih
-    case _ ih1 =>
-      constructor; assumption
-    case _ A z s =>
-      apply ParRed.nrec_zero (z := z) (s' := s)
-      case _ =>
-        apply ParRed.refl
-      case _ =>
-        apply ParRed.refl
-    case _ =>
-      apply ParRed.nrec_succ; apply ParRed.refl; apply ParRed.refl; apply ParRed.refl
-    case _ h1 ih1 =>
-      apply ParRed.nrec; apply ih1; apply ParRed.refl; apply ParRed.refl
-    case _ h1 ih1 =>
-      apply ParRed.nrec (ParRed.refl) ih1 (ParRed.refl)
-    case _ =>
-      apply ParRed.nrec (ParRed.refl) (ParRed.refl); assumption
-    case _ h ih =>
-      apply ParRed.inl ih
-    case _ h ih =>
-      apply ParRed.inr ih
+--   theorem seq_implies_par {t t'} : t ~> t' -> t ~p> t' := by
+--     intro h; induction h
+--     case beta => apply ParRed.beta ParRed.refl ParRed.refl
+--     case app1 r ih => apply ParRed.app ih ParRed.refl
+--     case app2 r ih => apply ParRed.app ParRed.refl ih
+--     case lam r ih => apply ParRed.lam ih
+--     case _ ih1 =>
+--       constructor; assumption
+--     case _ A z s =>
+--       apply ParRed.nrec_zero (z := z) (s' := s)
+--       case _ =>
+--         apply ParRed.refl
+--       case _ =>
+--         apply ParRed.refl
+--     case _ =>
+--       apply ParRed.nrec_succ; apply ParRed.refl; apply ParRed.refl; apply ParRed.refl
+--     case _ h1 ih1 =>
+--       apply ParRed.nrec; apply ih1; apply ParRed.refl; apply ParRed.refl
+--     case _ h1 ih1 =>
+--       apply ParRed.nrec (ParRed.refl) ih1 (ParRed.refl)
+--     case _ =>
+--       apply ParRed.nrec (ParRed.refl) (ParRed.refl); assumption
+--     case _ h ih =>
+--       apply ParRed.inl ih
+--     case _ h ih =>
+--       apply ParRed.inr ih
 
-  theorem seqs_implies_pars {t t'} : t ~>* t' -> t ~p>* t' := by
-    intro h; induction h
-    case _ => apply Star.refl
-    case _ y z r1 r2 ih =>
-      replace r2 := seq_implies_par r2
-      apply Star.step ih r2
+--   theorem seqs_implies_pars {t t'} : t ~>* t' -> t ~p>* t' := by
+--     intro h; induction h
+--     case _ => apply Star.refl
+--     case _ y z r1 r2 ih =>
+--       replace r2 := seq_implies_par r2
+--       apply Star.step ih r2
 
-  theorem par_implies_seqs {t t'} : t ~p> t' -> t ~>* t' := by
-    intro h; induction h
-    case var => apply Star.refl
-    case beta A b b' q q' r1 r2 ih1 ih2 =>
-      have lem : (:λ[A] b) ~>* (:λ[A] b') := by
-        apply Star.congr1 (Term.lam A) (@Red.lam A) ih1
-      apply Star.trans
-      apply Star.congr2 Term.app Red.app1 Red.app2 lem ih2
-      apply Star.step Star.refl
-      apply Red.beta
-    case app f f' a a' r1 r2 ih1 ih2 =>
-      apply Star.congr2 Term.app Red.app1 Red.app2 ih1 ih2
-    case lam t t' A r ih =>
-      apply Star.congr1 (Term.lam A) (@Red.lam A) ih
-    case _ =>
-      constructor
-    case _ ih =>
-      apply Star.congr1; intro t t'; intro h1; apply Red.succ h1
-      apply ih
-    case _ z z' s s' n n' A h1 h2 h3 ih1 ih2 ih3 =>
-      apply Star.congr3; intro t1 t2 t3 t1' j1; apply Red.nrec1 j1; intro t2 t3 t3' t2' j1; apply Red.nrec2 j1; intro t2 t3 t3' t3'' j1; apply Red.nrec3 j1
-      apply ih1; apply ih2; apply ih3
-    case _ z z' s s' A h1 h2 ih1 ih2 =>
-      apply Star.trans; apply Star.step; apply Star.refl; apply Red.nrec_zero; apply ih1
-    case _ z z' s s' n n' A h1 h2 h3 ih1 ih2 ih3 =>
-      apply Star.trans (y := s :@ Term.nrec A z s n); apply Star.step; apply Star.refl; apply Red.nrec_succ;
-      apply Star.trans (y := s :@ (Term.nrec A z' s' n')); apply Star.congr2; intro t1 t2 t1' j1
-      apply Red.app1 j1; intro t1 t2 t2' j1; apply Red.app2 j1; apply Star.refl; apply Star.congr3; intro t1 t2 t3 t1' j1; apply Red.nrec1 j1
-      intro t1 t2 t3 t2' j1; apply Red.nrec2 j1; intro t1 t2 t3 t3' j1; apply Red.nrec3 j1; apply ih1; apply ih2; apply ih3
-      apply Star.congr2; intro t1 t2 t1' j1; apply Red.app1 j1; intro t1 t2 t2' j1; apply Red.app2 j1; apply ih2; apply Star.refl
-    case _ h ih =>
-      apply Star.congr1; intro t t'; intro h1; apply Red.inl h1
-      apply ih
-    case _ h ih =>
-      apply Star.congr1; intro t t'; intro h1; apply Red.inr h1
-      apply ih
+--   theorem par_implies_seqs {t t'} : t ~p> t' -> t ~>* t' := by
+--     intro h; induction h
+--     case var => apply Star.refl
+--     case beta A b b' q q' r1 r2 ih1 ih2 =>
+--       have lem : (:λ[A] b) ~>* (:λ[A] b') := by
+--         apply Star.congr1 (Term.lam A) (@Red.lam A) ih1
+--       apply Star.trans
+--       apply Star.congr2 Term.app Red.app1 Red.app2 lem ih2
+--       apply Star.step Star.refl
+--       apply Red.beta
+--     case app f f' a a' r1 r2 ih1 ih2 =>
+--       apply Star.congr2 Term.app Red.app1 Red.app2 ih1 ih2
+--     case lam t t' A r ih =>
+--       apply Star.congr1 (Term.lam A) (@Red.lam A) ih
+--     case _ =>
+--       constructor
+--     case _ ih =>
+--       apply Star.congr1; intro t t'; intro h1; apply Red.succ h1
+--       apply ih
+--     case _ z z' s s' n n' A h1 h2 h3 ih1 ih2 ih3 =>
+--       apply Star.congr3; intro t1 t2 t3 t1' j1; apply Red.nrec1 j1; intro t2 t3 t3' t2' j1; apply Red.nrec2 j1; intro t2 t3 t3' t3'' j1; apply Red.nrec3 j1
+--       apply ih1; apply ih2; apply ih3
+--     case _ z z' s s' A h1 h2 ih1 ih2 =>
+--       apply Star.trans; apply Star.step; apply Star.refl; apply Red.nrec_zero; apply ih1
+--     case _ z z' s s' n n' A h1 h2 h3 ih1 ih2 ih3 =>
+--       apply Star.trans (y := s :@ Term.nrec A z s n); apply Star.step; apply Star.refl; apply Red.nrec_succ;
+--       apply Star.trans (y := s :@ (Term.nrec A z' s' n')); apply Star.congr2; intro t1 t2 t1' j1
+--       apply Red.app1 j1; intro t1 t2 t2' j1; apply Red.app2 j1; apply Star.refl; apply Star.congr3; intro t1 t2 t3 t1' j1; apply Red.nrec1 j1
+--       intro t1 t2 t3 t2' j1; apply Red.nrec2 j1; intro t1 t2 t3 t3' j1; apply Red.nrec3 j1; apply ih1; apply ih2; apply ih3
+--       apply Star.congr2; intro t1 t2 t1' j1; apply Red.app1 j1; intro t1 t2 t2' j1; apply Red.app2 j1; apply ih2; apply Star.refl
+--     case _ h ih =>
+--       apply Star.congr1; intro t t'; intro h1; apply Red.inl h1
+--       apply ih
+--     case _ h ih =>
+--       apply Star.congr1; intro t t'; intro h1; apply Red.inr h1
+--       apply ih
 
-  theorem pars_implies_seqs {t t'} : t ~p>* t' -> t ~>* t' := by
-    intro h; induction h
-    case _ => apply Star.refl
-    case _ y z r1 r2 ih =>
-      replace r2 := par_implies_seqs r2
-      apply Star.trans ih r2
+--   theorem pars_implies_seqs {t t'} : t ~p>* t' -> t ~>* t' := by
+--     intro h; induction h
+--     case _ => apply Star.refl
+--     case _ y z r1 r2 ih =>
+--       replace r2 := par_implies_seqs r2
+--       apply Star.trans ih r2
 
-  theorem pars_action_lift : t ~p>* t' -> .su t ~ps>* .su t' := by
-    intro r; induction r
-    case _ => apply Star.refl
-    case _ r1 r2 ih =>
-      apply Star.step ih
-      apply ActionRed.su r2
+--   theorem pars_action_lift : t ~p>* t' -> .su t ~ps>* .su t' := by
+--     intro r; induction r
+--     case _ => apply Star.refl
+--     case _ r1 r2 ih =>
+--       apply Star.step ih
+--       apply ActionRed.su r2
 
-  theorem seqs_action_lift : t ~>* t' -> .su t ~s>* .su t' := by
-    intro r; induction r
-    case _ => apply Star.refl
-    case _ r1 r2 ih =>
-      apply Star.step ih
-      apply ActionRed.su r2
+--   theorem seqs_action_lift : t ~>* t' -> .su t ~s>* .su t' := by
+--     intro r; induction r
+--     case _ => apply Star.refl
+--     case _ r1 r2 ih =>
+--       apply Star.step ih
+--       apply ActionRed.su r2
 
-  theorem seqs_action_destruct : a ~s>* .su t' -> ∃ t, a = .su t ∧ t ~>* t' := by
-    intro r
-    generalize zdef : Subst.Action.su t' = z at r
-    induction r generalizing t'
-    case _ =>
-      subst zdef; exists t'; simp
-      apply Star.refl
-    case _ r1 r2 ih =>
-      subst zdef; cases r2
-      case _ t r2 =>
-        replace ih := @ih t rfl
-        cases ih; case _ z ih =>
-        cases ih; case _ e ih =>
-        subst e; exists z; apply And.intro rfl
-        apply Star.step ih r2
+--   theorem seqs_action_destruct : a ~s>* .su t' -> ∃ t, a = .su t ∧ t ~>* t' := by
+--     intro r
+--     generalize zdef : Subst.Action.su t' = z at r
+--     induction r generalizing t'
+--     case _ =>
+--       subst zdef; exists t'; simp
+--       apply Star.refl
+--     case _ r1 r2 ih =>
+--       subst zdef; cases r2
+--       case _ t r2 =>
+--         replace ih := @ih t rfl
+--         cases ih; case _ z ih =>
+--         cases ih; case _ e ih =>
+--         subst e; exists z; apply And.intro rfl
+--         apply Star.step ih r2
 
-  theorem pars_action_iff_seqs_action : t ~ps>* t' <-> t ~s>* t' := by
-    apply Iff.intro
-    case _ =>
-      intro h; induction h
-      case _ => apply Star.refl
-      case _ r1 r2 ih =>
-        cases r2
-        case _ r2 =>
-          have lem := seqs_action_destruct ih
-          cases lem; case _ z lem =>
-          cases lem; case _ e lem =>
-          subst e
-          replace r2 := par_implies_seqs r2
-          apply Star.trans ih
-          apply seqs_action_lift r2
-        case _ => apply ih
-    case _ =>
-      intro h; induction h
-      case _ => apply Star.refl
-      case _ r1 r2 ih =>
-        cases r2
-        case _ r2 =>
-          replace r1 := seqs_action_destruct r1
-          cases r1; case _ z r1 =>
-          cases r1; case _ e r1 =>
-          subst e; replace r2 := Star.step r1 r2
-          replace r2 := seqs_implies_pars r2
-          apply pars_action_lift r2
-        case _ => apply ih
+--   theorem pars_action_iff_seqs_action : t ~ps>* t' <-> t ~s>* t' := by
+--     apply Iff.intro
+--     case _ =>
+--       intro h; induction h
+--       case _ => apply Star.refl
+--       case _ r1 r2 ih =>
+--         cases r2
+--         case _ r2 =>
+--           have lem := seqs_action_destruct ih
+--           cases lem; case _ z lem =>
+--           cases lem; case _ e lem =>
+--           subst e
+--           replace r2 := par_implies_seqs r2
+--           apply Star.trans ih
+--           apply seqs_action_lift r2
+--         case _ => apply ih
+--     case _ =>
+--       intro h; induction h
+--       case _ => apply Star.refl
+--       case _ r1 r2 ih =>
+--         cases r2
+--         case _ r2 =>
+--           replace r1 := seqs_action_destruct r1
+--           cases r1; case _ z r1 =>
+--           cases r1; case _ e r1 =>
+--           subst e; replace r2 := Star.step r1 r2
+--           replace r2 := seqs_implies_pars r2
+--           apply pars_action_lift r2
+--         case _ => apply ih
 
-  theorem subst_arg {t} {σ σ' : Subst Term} :
-    (∀ x, σ x ~s> σ' x) ->
-    t[σ] ~>* t[σ']
-  := by
-    intro h
-    induction t generalizing σ σ' <;> simp at *
-    case _ x =>
-      generalize zdef : σ x = z at *
-      generalize wdef : σ' x = w at *
-      cases z
-      case _ t =>
-        replace h := h x; rw [zdef] at h
-        rw [wdef] at h; cases h; simp
-        apply Star.refl
-      case _ t =>
-        replace h := h x; rw [zdef] at h
-        rw [wdef] at h; cases h; simp
-        case _ t' r =>
-        apply Star.step Star.refl r
-    case _ ih1 ih2 =>
-      apply Star.congr2 Term.app Red.app1 Red.app2 (ih1 h) (ih2 h)
-    case _ A a ih =>
-      have lem := subst_red_lift h
-      replace ih := ih lem
-      have lem2 := Star.congr1 (t1 := a[σ.lift]) (t1' := a[σ'.lift]) (:λ[A] ·) (@Red.lam A) ih
-      simp at lem2; apply lem2
-    case _ =>
-      apply Star.refl
-    case _ t ih =>
-      apply Star.congr1; intro t t' h2; apply Red.succ h2
-      apply ih h
-    case _ A t t' t'' ih1 ih2 ih3 =>
-      apply Star.congr3; intro t1 t2 t3 t1' h1; apply Red.nrec1 h1; intro t1 t2 t3 t2' h2; apply Red.nrec2 h2
-      intro t1 t2 t3 t3' h1; apply Red.nrec3 h1; apply ih1 h; apply ih2 h; apply ih3 h
-    case _ t ih =>
-      apply Star.congr1; intro t t' h2; apply Red.inl h2
-      apply ih h
-    case _ t ih =>
-      apply Star.congr1; intro t t' h2; apply Red.inr h2
-      apply ih h
+--   theorem subst_arg {t} {σ σ' : Subst Term} :
+--     (∀ x, σ x ~s> σ' x) ->
+--     t[σ] ~>* t[σ']
+--   := by
+--     intro h
+--     induction t generalizing σ σ' <;> simp at *
+--     case _ x =>
+--       generalize zdef : σ x = z at *
+--       generalize wdef : σ' x = w at *
+--       cases z
+--       case _ t =>
+--         replace h := h x; rw [zdef] at h
+--         rw [wdef] at h; cases h; simp
+--         apply Star.refl
+--       case _ t =>
+--         replace h := h x; rw [zdef] at h
+--         rw [wdef] at h; cases h; simp
+--         case _ t' r =>
+--         apply Star.step Star.refl r
+--     case _ ih1 ih2 =>
+--       apply Star.congr2 Term.app Red.app1 Red.app2 (ih1 h) (ih2 h)
+--     case _ A a ih =>
+--       have lem := subst_red_lift h
+--       replace ih := ih lem
+--       have lem2 := Star.congr1 (t1 := a[σ.lift]) (t1' := a[σ'.lift]) (:λ[A] ·) (@Red.lam A) ih
+--       simp at lem2; apply lem2
+--     case _ =>
+--       apply Star.refl
+--     case _ t ih =>
+--       apply Star.congr1; intro t t' h2; apply Red.succ h2
+--       apply ih h
+--     case _ A t t' t'' ih1 ih2 ih3 =>
+--       apply Star.congr3; intro t1 t2 t3 t1' h1; apply Red.nrec1 h1; intro t1 t2 t3 t2' h2; apply Red.nrec2 h2
+--       intro t1 t2 t3 t3' h1; apply Red.nrec3 h1; apply ih1 h; apply ih2 h; apply ih3 h
+--     case _ t ih =>
+--       apply Star.congr1; intro t t' h2; apply Red.inl h2
+--       apply ih h
+--     case _ t ih =>
+--       apply Star.congr1; intro t t' h2; apply Red.inr h2
+--       apply ih h
 
-  theorem confluence {s t1 t2} : s ~>* t1 -> s ~>* t2 -> ∃ t, t1 ~>* t ∧ t2 ~>* t := by
-    intro h1 h2
-    have lem1 := seqs_implies_pars h1
-    have lem2 := seqs_implies_pars h2
-    have lem3 := HasConfluence.confluence lem1 lem2
-    cases lem3; case _ w lem3 =>
-    have lem4 := pars_implies_seqs lem3.1
-    have lem5 := pars_implies_seqs lem3.2
-    exists w
+--   theorem confluence {s t1 t2} : s ~>* t1 -> s ~>* t2 -> ∃ t, t1 ~>* t ∧ t2 ~>* t := by
+--     intro h1 h2
+--     have lem1 := seqs_implies_pars h1
+--     have lem2 := seqs_implies_pars h2
+--     have lem3 := HasConfluence.confluence lem1 lem2
+--     cases lem3; case _ w lem3 =>
+--     have lem4 := pars_implies_seqs lem3.1
+--     have lem5 := pars_implies_seqs lem3.2
+--     exists w
 
-  instance : Substitutive Red where
-    subst := subst
+--   instance : Substitutive Red where
+--     subst := subst
 
-  instance : HasConfluence Red where
-    confluence := confluence
+--   instance : HasConfluence Red where
+--     confluence := confluence
 
-  theorem preservation_of_neutral_step : Neutral t -> t ~> t' -> Neutral t'
-  | .app fn, .app1 r => .app (preservation_of_neutral_step fn r)
-  | .app fn, .app2 r => .app fn
-  | .nrec nn, .nrec1 r => .nrec nn
-  | .nrec nn, .nrec2 r => .nrec nn
-  | .nrec nn, .nrec3 r => .nrec (preservation_of_neutral_step nn r)
+--   theorem preservation_of_neutral_step : Neutral t -> t ~> t' -> Neutral t'
+--   | .app fn, .app1 r => .app (preservation_of_neutral_step fn r)
+--   | .app fn, .app2 r => .app fn
+--   | .nrec nn, .nrec1 r => .nrec nn
+--   | .nrec nn, .nrec2 r => .nrec nn
+--   | .nrec nn, .nrec3 r => .nrec (preservation_of_neutral_step nn r)
 
-  theorem preservation_of_neutral : Neutral t -> t ~>* t' -> Neutral t' := by
-    intro h r
-    induction r
-    case _ => apply h
-    case _ r1 r2 ih =>
-      apply preservation_of_neutral_step ih r2
-end Red
+--   theorem preservation_of_neutral : Neutral t -> t ~>* t' -> Neutral t' := by
+--     intro h r
+--     induction r
+--     case _ => apply h
+--     case _ r1 r2 ih =>
+--       apply preservation_of_neutral_step ih r2
+--end Red
